Move covered

src/opt/SimMemory.v
@@ -21,6 +21,8 @@ Require Import Local.
 Require Import Thread.
 Require Import Configuration.
 
+Require Import Cover.
+
 Set Implicit Arguments.
 
 
@@ -69,20 +71,6 @@ Lemma sim_message_message_same_kind
 Proof.
   inv SIM; econs.
 Qed.
-
-Inductive covered (loc:Loc.t) (ts:Time.t) (mem:Memory.t): Prop :=
-| covered_intro
-    from to msg
-    (GET: Memory.get loc to mem = Some (from, msg))
-    (ITV: Interval.mem (from, to) ts)
-.
-
-Inductive covered_half (loc: Loc.t) (ts: Time.t) (mem: Memory.t): Prop :=
-| covered_half_intro
-    from to
-    (GET: Memory.get loc to mem = Some (from, Message.half))
-    (ITV: Interval.mem (from, to) ts)
-.
 
 Inductive sim_memory (mem_src mem_tgt:Memory.t): Prop :=
 | sim_memory_intro
@@ -279,120 +267,6 @@ Proof.
   inv MAX_SRC. inv MAX_TGT.
   exploit sim_memory_max_full_timemap; try exact SIM; eauto. i.
   subst. ss.
-Qed.
-
-Lemma covered_disjoint
-      mem1 mem2 loc from to
-      (COVER: forall loc ts, covered loc ts mem1 -> covered loc ts mem2)
-      (DISJOINT: forall to2 from2 msg2
-                   (GET2: Memory.get loc to2 mem2 = Some (from2, msg2)),
-          Interval.disjoint (from, to) (from2, to2)):
-  forall to2 from2 msg2
-    (GET2: Memory.get loc to2 mem1 = Some (from2, msg2)),
-    Interval.disjoint (from, to) (from2, to2).
-Proof.
-  ii. exploit COVER; eauto.
-  { econs; eauto. }
-  i. inv x0. eapply DISJOINT; eauto.
-Qed.
-
-Lemma get_disjoint_covered_disjoint
-      mem loc from to:
-  (forall t f m, Memory.get loc t mem = Some (f, m) -> Interval.disjoint (from, to) (f, t)) ->
-  (forall ts, covered loc ts mem -> ~ Interval.mem (from, to) ts).
-Proof.
-  ii. inv H0. eapply H; eauto.
-Qed.
-
-Lemma covered_disjoint_get_disjoint
-      mem loc from to:
-  (forall ts, covered loc ts mem -> ~ Interval.mem (from, to) ts) ->
-  (forall t f m, Memory.get loc t mem = Some (f, m) -> Interval.disjoint (from, to) (f, t)).
-Proof.
-  ii. eapply H; eauto. econs; eauto.
-Qed.
-
-Lemma add_covered
-      mem2 mem1 loc from to msg
-      l t
-      (ADD: Memory.add mem1 loc from to msg mem2):
-  covered l t mem2 <->
-  covered l t mem1 \/ (l = loc /\ Interval.mem (from, to) t).
-Proof.
-  econs; i.
-  - inv H. revert GET. erewrite Memory.add_o; eauto. condtac; ss.
-    + des. subst. i. inv GET. auto.
-    + left. econs; eauto.
-  - des.
-    + inv H. econs; eauto.
-      erewrite Memory.add_o; eauto. condtac; ss; eauto.
-      des. subst. exploit Memory.add_get0; eauto. i. des. congr.
-    + subst. econs; eauto. erewrite Memory.add_o; eauto. condtac; ss.
-      des; congr.
-Qed.
-
-Lemma split_covered
-      mem2 mem1 loc ts1 ts2 ts3 msg2 msg3
-      l t
-      (SPLIT: Memory.split mem1 loc ts1 ts2 ts3 msg2 msg3 mem2):
-  covered l t mem2 <-> covered l t mem1.
-Proof.
-  econs; i.
-  - exploit Memory.split_get0; eauto. i. des.
-    inv H. revert GET3. erewrite Memory.split_o; eauto. repeat condtac; ss.
-    + des. subst. i. inv GET3. econs; eauto.
-      eapply Interval.le_mem; eauto. econs; [refl|].
-      inv SPLIT. inv SPLIT0. left. auto.
-    + guardH o. des. subst. i. inv GET3. econs; eauto.
-      eapply Interval.le_mem; eauto. econs; [|refl].
-      inv SPLIT. inv SPLIT0. left. auto.
-    + i. econs; eauto.
-  - exploit Memory.split_get0; eauto. i. des.
-    inv H.
-    destruct (loc_ts_eq_dec (l, to) (loc, ts3)); ss.
-    + des. subst. rewrite GET0 in GET3. inv GET3.
-      destruct (Time.le_lt_dec t ts2).
-      * econs.
-        { instantiate (2 := from). instantiate (2 := ts2).
-          erewrite Memory.split_o; eauto. condtac; ss.
-          des; congr.
-        }
-        { inv ITV. econs; ss. }
-      * econs.
-        { instantiate (2 := ts2). instantiate (2 := ts3).
-          erewrite Memory.split_o; eauto. repeat condtac; ss.
-          - des. subst. inv SPLIT. inv SPLIT0.
-            exfalso. eapply Time.lt_strorder. eauto.
-          - guardH o. des; congr.
-        }
-        { inv ITV. econs; ss. }
-    + econs; eauto. erewrite Memory.split_o; eauto.
-      repeat condtac; ss; eauto.
-      * guardH o. des. subst. congr.
-      * guardH o. guardH o0. des. subst.
-        unguardH o. des; congr.
-Qed.
-
-Lemma lower_covered
-      mem2 mem1 loc from to msg1 msg2
-      l t
-      (LOWER: Memory.lower mem1 loc from to msg1 msg2 mem2):
-  covered l t mem2 <-> covered l t mem1.
-Proof.
-  econs; i.
-  - inv H. revert GET. erewrite Memory.lower_o; eauto. condtac; ss.
-    + des. subst. i. inv GET. econs; eauto.
-      hexploit Memory.lower_get0; eauto. i. des. eauto.
-    + i. econs; eauto.
-  - exploit Memory.lower_get0; eauto. i. des.
-    inv H.
-    destruct (loc_ts_eq_dec (l, to0) (loc, to)); ss.
-    + des. subst. econs; cycle 1; eauto.
-      erewrite Memory.lower_o; eauto. condtac; [|by des].
-      rewrite GET in GET1. inv GET1. eauto.
-    + econs; eauto.
-      erewrite Memory.lower_o; eauto. rewrite GET1. condtac; ss.
-      des; congr.
 Qed.
 
 Lemma split_sim_memory
@@ -866,15 +740,4 @@ Proof.
     etrans; try exact x1.
     eapply TimeFacts.lt_le_lt; try exact TS2. ss.
   - apply (x3 to); econs; ss; try refl. econs. ss.
-Qed.
-
-Lemma cap_cover
-      promises mem1 mem2 loc ts
-      (CAP: Memory.cap promises mem1 mem2)
-      (COVER: covered loc ts mem1):
-  covered loc ts mem2.
-Proof.
-  inv CAP. inv COVER.
-  exploit SOUND; eauto. i.
-  econs; eauto.
 Qed.
