src/opt/SimPromises.v
@@ -22,9 +22,10 @@ Require Import Local.
 Require Import Thread.
 Require Import Configuration.
 
-Require Import SimMemory.
 Require Import MemorySplit.
 Require Import MemoryMerge.
+Require Import Cover.
+Require Import SimMemory.
 
 Set Implicit Arguments.
 
