src/prop/Cover.v
@@ -1,0 +1,158 @@
+Require Import RelationClasses.
+
+Require Import sflib.
+From Paco Require Import paco.
+
+Require Import Axioms.
+Require Import Basic.
+Require Import DataStructure.
+Require Import DenseOrder.
+Require Import Event.
+Require Import Time.
+Require Import Language.
+Require Import View.
+Require Import Cell.
+Require Import Memory.
+Require Import MemoryFacts.
+
+Set Implicit Arguments.
+
+
+Inductive covered (loc:Loc.t) (ts:Time.t) (mem:Memory.t): Prop :=
+| covered_intro
+    from to msg
+    (GET: Memory.get loc to mem = Some (from, msg))
+    (ITV: Interval.mem (from, to) ts)
+.
+
+Inductive covered_half (loc: Loc.t) (ts: Time.t) (mem: Memory.t): Prop :=
+| covered_half_intro
+    from to
+    (GET: Memory.get loc to mem = Some (from, Message.half))
+    (ITV: Interval.mem (from, to) ts)
+.
+
+Lemma covered_disjoint
+      mem1 mem2 loc from to
+      (COVER: forall loc ts, covered loc ts mem1 -> covered loc ts mem2)
+      (DISJOINT: forall to2 from2 msg2
+                   (GET2: Memory.get loc to2 mem2 = Some (from2, msg2)),
+          Interval.disjoint (from, to) (from2, to2)):
+  forall to2 from2 msg2
+    (GET2: Memory.get loc to2 mem1 = Some (from2, msg2)),
+    Interval.disjoint (from, to) (from2, to2).
+Proof.
+  ii. exploit COVER; eauto.
+  { econs; eauto. }
+  i. inv x0. eapply DISJOINT; eauto.
+Qed.
+
+Lemma get_disjoint_covered_disjoint
+      mem loc from to:
+  (forall t f m, Memory.get loc t mem = Some (f, m) -> Interval.disjoint (from, to) (f, t)) ->
+  (forall ts, covered loc ts mem -> ~ Interval.mem (from, to) ts).
+Proof.
+  ii. inv H0. eapply H; eauto.
+Qed.
+
+Lemma covered_disjoint_get_disjoint
+      mem loc from to:
+  (forall ts, covered loc ts mem -> ~ Interval.mem (from, to) ts) ->
+  (forall t f m, Memory.get loc t mem = Some (f, m) -> Interval.disjoint (from, to) (f, t)).
+Proof.
+  ii. eapply H; eauto. econs; eauto.
+Qed.
+
+Lemma add_covered
+      mem2 mem1 loc from to msg
+      l t
+      (ADD: Memory.add mem1 loc from to msg mem2):
+  covered l t mem2 <->
+  covered l t mem1 \/ (l = loc /\ Interval.mem (from, to) t).
+Proof.
+  econs; i.
+  - inv H. revert GET. erewrite Memory.add_o; eauto. condtac; ss.
+    + des. subst. i. inv GET. auto.
+    + left. econs; eauto.
+  - des.
+    + inv H. econs; eauto.
+      erewrite Memory.add_o; eauto. condtac; ss; eauto.
+      des. subst. exploit Memory.add_get0; eauto. i. des. congr.
+    + subst. econs; eauto. erewrite Memory.add_o; eauto. condtac; ss.
+      des; congr.
+Qed.
+
+Lemma split_covered
+      mem2 mem1 loc ts1 ts2 ts3 msg2 msg3
+      l t
+      (SPLIT: Memory.split mem1 loc ts1 ts2 ts3 msg2 msg3 mem2):
+  covered l t mem2 <-> covered l t mem1.
+Proof.
+  econs; i.
+  - exploit Memory.split_get0; eauto. i. des.
+    inv H. revert GET3. erewrite Memory.split_o; eauto. repeat condtac; ss.
+    + des. subst. i. inv GET3. econs; eauto.
+      eapply Interval.le_mem; eauto. econs; [refl|].
+      inv SPLIT. inv SPLIT0. left. auto.
+    + guardH o. des. subst. i. inv GET3. econs; eauto.
+      eapply Interval.le_mem; eauto. econs; [|refl].
+      inv SPLIT. inv SPLIT0. left. auto.
+    + i. econs; eauto.
+  - exploit Memory.split_get0; eauto. i. des.
+    inv H.
+    destruct (loc_ts_eq_dec (l, to) (loc, ts3)); ss.
+    + des. subst. rewrite GET0 in GET3. inv GET3.
+      destruct (Time.le_lt_dec t ts2).
+      * econs.
+        { instantiate (2 := from). instantiate (2 := ts2).
+          erewrite Memory.split_o; eauto. condtac; ss.
+          des; congr.
+        }
+        { inv ITV. econs; ss. }
+      * econs.
+        { instantiate (2 := ts2). instantiate (2 := ts3).
+          erewrite Memory.split_o; eauto. repeat condtac; ss.
+          - des. subst. inv SPLIT. inv SPLIT0.
+            exfalso. eapply Time.lt_strorder. eauto.
+          - guardH o. des; congr.
+        }
+        { inv ITV. econs; ss. }
+    + econs; eauto. erewrite Memory.split_o; eauto.
+      repeat condtac; ss; eauto.
+      * guardH o. des. subst. congr.
+      * guardH o. guardH o0. des. subst.
+        unguardH o. des; congr.
+Qed.
+
+Lemma lower_covered
+      mem2 mem1 loc from to msg1 msg2
+      l t
+      (LOWER: Memory.lower mem1 loc from to msg1 msg2 mem2):
+  covered l t mem2 <-> covered l t mem1.
+Proof.
+  econs; i.
+  - inv H. revert GET. erewrite Memory.lower_o; eauto. condtac; ss.
+    + des. subst. i. inv GET. econs; eauto.
+      hexploit Memory.lower_get0; eauto. i. des. eauto.
+    + i. econs; eauto.
+  - exploit Memory.lower_get0; eauto. i. des.
+    inv H.
+    destruct (loc_ts_eq_dec (l, to0) (loc, to)); ss.
+    + des. subst. econs; cycle 1; eauto.
+      erewrite Memory.lower_o; eauto. condtac; [|by des].
+      rewrite GET in GET1. inv GET1. eauto.
+    + econs; eauto.
+      erewrite Memory.lower_o; eauto. rewrite GET1. condtac; ss.
+      des; congr.
+Qed.
+
+Lemma cap_cover
+      promises mem1 mem2 loc ts
+      (CAP: Memory.cap promises mem1 mem2)
+      (COVER: covered loc ts mem1):
+  covered loc ts mem2.
+Proof.
+  inv CAP. inv COVER.
+  exploit SOUND; eauto. i.
+  econs; eauto.
+Qed.
